



J) IS
$$T(x) = (1 + x_k)$$
 a linear transformation?

 $T(0) = (1)$ So no! violates c)

Upshot Linear transformations are special.

Note Look at the 2.1 Example 9 for application to $1 = 2$ page Rank

Use matrix to describe the users transition attix."

In If $T: \mathbb{R}^n \to \mathbb{R}^p$ is a linear transformation

represented by px m matrix A and $S: \mathbb{R}^p \to \mathbb{R}^n$ is represented by BA, i.e. $S(T(x)) = BAx$ for all $x \in \mathbb{R}^n$.

Inverses

Eq. $(\frac{1}{3} + \frac{1}{4})(\frac{x_1}{4}) = (\frac{x_1}{3} + \frac{1}{4}x_2)$
 $(\frac{1}{4} + \frac{1}{4})(\frac{x_1}{4}) = (\frac{x_1}{3} + \frac{1}{4}x_2)$

Can be find a matrix A such that

 $A(x_1 + 2x_2) = (\frac{x_1}{3})(\frac{x_1}{3}) = (\frac{x_1}{3})(\frac{x_2}{3})(\frac{x_1}{3})(\frac{x_2}{3})(\frac{x_1}{3})(\frac{x_2}{3})(\frac{x_1}{3})(\frac{x_2}{3})(\frac{x_1}{3})(\frac{x_2}{3})(\frac{x_1}{3})(\frac{x_2}{3})(\frac{x_1}{3})(\frac{x_2}{3})(\frac{x_1}{3})(\frac{x_2}{3})(\frac{x_1}{3})(\frac{x_2}{3})(\frac{x_1}{3})(\frac{x_2}{3})(\frac{x_1}{3})(\frac{x_2}{3})(\frac{x_1}{3})(\frac{x_2}{3})(\frac{x_1}{3})(\frac{x_2}{3})(\frac{x_1}{3})(\frac{x_2}{3})(\frac{x_1}{3})(\frac{x_1}{3})(\frac{x_2}{3})(\frac{x_1}{3})(\frac{x_1}{3})(\frac{x_2}{3})(\frac{x_1}{3})(\frac{x_2}{3})(\frac{x_1}{3})(\frac{x_2}{3})(\frac{x_1}{3})(\frac{x_1}{3})(\frac{x_2}{3})(\frac{x_1}{3})(\frac{x_1}{3})(\frac{x_2}{3})(\frac{x_1}{3})$

Say
$$\begin{cases} X_1 + 2X_2 = y_1 \\ 3X_1 + 4X_2 = y_2 \end{cases}$$
 how can be write X_1, X_2 in terms of $y_1, y_2 = y_2$

$$\begin{cases} X_1 + 2X_2 = y_1 \\ 3X_1 + 4X_2 = y_2 \end{cases}$$

$$\begin{cases} X_1 + 2X_2 = y_1 \\ X_2 = \frac{1}{2}y_1 - \frac{1}{2}y_2 \end{cases}$$

$$\begin{cases} X_1 + 2X_2 = y_2 \\ X_2 = \frac{1}{2}y_1 - \frac{1}{2}y_2 \end{cases}$$

$$\begin{cases} X_1 + 2X_2 = y_1 \\ \frac{1}{2} - \frac{1}{2} \end{cases}$$

$$\begin{cases} X_1 + 2X_2 = y_2 \\ \frac{1}{2} - \frac{1}{2} \end{cases}$$

$$\begin{cases} X_1 + 2X_2 = \frac{1}{2}y_1 - \frac{1}{2}y_2 \\ \frac{1}{2} - \frac{1}{2} \end{cases}$$

$$\begin{cases} X_1 + 2X_2 = \frac{1}{2}y_1 - \frac{1}{2}y_2 \\ \frac{1}{2} - \frac{1}{2} \end{cases}$$

$$\begin{cases} X_1 + 2X_2 = y_1 \\ \frac{1}{2} - \frac{1}{2} \end{cases}$$

$$\begin{cases} X_1 + 2X_2 = y_1 \\ \frac{1}{2} - \frac{1}{2} \end{cases}$$

$$\begin{cases} X_1 + 2X_2 = y_1 \\ \frac{1}{2} - \frac{1}{2} \end{cases}$$

$$\begin{cases} X_1 + 2X_2 = y_1 \\ \frac{1}{2} - \frac{1}{2} \end{cases}$$

$$\begin{cases} X_1 + 2X_2 = y_1 \\ \frac{1}{2} - \frac{1}{2} \end{cases}$$

$$\begin{cases} X_1 + 2X_2 = y_1 \\ \frac{1}{2} - \frac{1}{2} \end{cases}$$

$$\begin{cases} X_1 + 2X_2 = y_1 \\ \frac{1}{2} - \frac{1}{2} \end{cases}$$

$$\begin{cases} X_1 + 2X_2 = y_1 \\ \frac{1}{2} - \frac{1}{2} \end{cases}$$

$$\begin{cases} X_1 + 2X_2 = y_1 \\ \frac{1}{2} - \frac{1}{2} \end{cases}$$

$$\begin{cases} X_1 + 2X_2 = y_1 \\ \frac{1}{2} - \frac{1}{2} \end{cases}$$

$$\begin{cases} X_1 + 2X_2 = y_1 \\ \frac{1}{2} - \frac{1}{2} \end{cases}$$

$$\begin{cases} X_1 + 2X_2 = y_1 \\ \frac{1}{2} - \frac{1}{2} \end{cases}$$

$$\begin{cases} X_1 + 2X_2 = y_1 \\ \frac{1}{2} - \frac{1}{2} \end{cases}$$

$$\begin{cases} X_1 + 2X_2 = y_1 \\ \frac{1}{2} - \frac{1}{2} \end{cases}$$

$$\begin{cases} X_1 + 2X_2 = y_1 \\ \frac{1}{2} - \frac{1}{2} \end{cases}$$

$$\begin{cases} X_1 + 2X_2 = y_1 \\ \frac{1}{2} - \frac{1}{2} \end{cases}$$

$$\begin{cases} X_1 + 2X_2 = y_1 \\ \frac{1}{2} - \frac{1}{2} \end{cases}$$

$$\begin{cases} X_1 + 2X_2 = y_1 \\ \frac{1}{2} - \frac{1}{2} \end{cases}$$

$$\begin{cases} X_1 + 2X_2 = y_1 \\ \frac{1}{2} - \frac{1}{2} \end{cases}$$

$$\begin{cases} X_1 + 2X_2 = y_1 \\ \frac{1}{2} - \frac{1}{2} \end{cases}$$

$$\begin{cases} X_1 + 2X_2 = y_1 \\ \frac{1}{2} - \frac{1}{2} \end{cases}$$

$$\begin{cases} X_1 + 2X_2 = y_1 \\ \frac{1}{2} - \frac{1}{2} \end{cases}$$

$$\begin{cases} X_1 + 2X_2 = y_1 \\ \frac{1}{2} - \frac{1}{2} \end{cases}$$

$$\begin{cases} X_1 + 2X_2 = y_1 \\ \frac{1}{2} - \frac{1}{2} \end{cases}$$

$$\begin{cases} X_1 + 2X_2 = y_1 \\ \frac{1}{2} - \frac{1}{2} \end{cases}$$

$$\begin{cases} X_1 + 2X_2 = y_1 \\ \frac{1}{2} - \frac{1}{2} \end{cases}$$

$$\begin{cases} X_1 + 2X_2 = y_1 \\ \frac{1}{2} - \frac{1}{2} \end{cases}$$

$$\begin{cases} X_1 + 2X_2 = y_1 \\ \frac{1}{2} - \frac{1}{2} \end{cases}$$

$$\begin{cases} X_1 + 2X_2 = y_1 \\ \frac{1}{2} - \frac{1}{2} \end{cases}$$

$$\begin{cases} X_1 + 2X_2 = y_1 \\ \frac{1}{2} - \frac{1}{2} \end{cases}$$

$$\begin{cases} X_1 + 2X_2 = y_1 \\ \frac{1}{2} - \frac{1}{2} \end{cases}$$

$$\begin{cases} X_1 + 2X_2 = y_1 \\ \frac{1}{2} - \frac{1}{2} \end{cases}$$

$$\begin{cases} X_1 + 2X_2 = y_1 \\ \frac{1}{2} - \frac{1}{2} \end{cases}$$

$$\begin{cases} X_1 + 2X_2 = y_1 \\ \frac{1}{2} - \frac{1}{2} \end{cases}$$

$$\begin{cases} X_1 + 2X_2 = y_1 \\ \frac{1}{2} - \frac{1}{2} \end{cases}$$

$$\begin{cases} X_1 + 2X_2 = y_1 \\ \frac{1}{2} - \frac{1}{2} \end{cases}$$

$$\begin{cases} X_1 + 2X_2 = y_1 \\ \frac{1}{2$$